\newpage
\begin{question}
Use the identify $\displaystyle\frac 1 {k(k+1)} = \frac 1 k - \frac 1 {k+1}$ and \textbf{telescoping} to compute $\displaystyle \sum_{k=1}^{n} \frac 1 {k(k+1)}$.

% Theorem Styles
\theoremstyle{remark}
\newtheorem*{note}{Note}
\begin{note}
$\displaystyle\sum_{j = 1} ^{n} a_{j} - a_{j-1} = a_{n} - a_{0}$, where $a_{0},a_{1},...,a_{n}$ is a sequence of real numbers. This type of sum is called telescoping.
\end{note}
\end{question}

\par\noindent\rule{\textwidth}{0.5pt}

\subsubsection*{Solutions}

Using the given identify formula, We can change of the sum as:
$$\sum_{k=1} ^n \frac 1 {k(k+1)} = \sum _{k=1} ^n \left ( \frac 1 k - \frac 1 {k + 1} \right )$$

\noindent
Then, we can rewrite the sum seperately as:
$$\sum _{k=1} ^n \left ( \frac 1 k - \frac 1 {k + 1} \right ) = \left ( \frac 1 1 - \frac 1 2 \right ) + \left ( \frac 1 2 - \frac 1 3 \right ) + \cdots + \left ( \frac 1 n - \frac 1 {n+1} \right )$$

\noindent
Only first and last terms are remain, and the sum of others are $0$. (This is the main property of telescoping sums)

\noindent
Finally, we get:
$$\sum _{k=1} ^n \frac 1 {k(k+1)} = \left ( \frac 1 1 - \frac 1 {n+1} \right ) = 1 - \frac 1 {n+1}$$