\begin{question}
Prove that
$$
\sum_{j=0}^n\left(-\frac{1}{2}\right)^j=\frac{2^{n+1}+(-1)^n}{3 \cdot 2^n}
$$
whenever $n$ is a nonnegative integer.
\end{question}

\par\noindent\rule{\textwidth}{0.5pt}

\subsubsection*{Solutions}

\begin{proof}
    We will prove by induction. If $n$ is $0$, then the both sides are equal to $1$. Next, we assume that the statement is true when $n = k$, then we have to prove that the statement is true when $n = k+1$.
    \begin{align*}
        \sum _{j = 0}^n \left( - \frac 1 2 \right) ^j
            &= \sum _{j=0}^{k} \left( - \frac 1 2 \right) ^j + \left( - \frac 1 2 \right) ^{k+1}\\
            &= \frac{2^{k+1} + (-1)^k}{3 \cdot 2^k} + (-1)^{k+1} \frac 1 {2 \times 2^{k}}\\
            &= \frac{2\cdot2^{k+1} + 2(-1)^k + 3(-1)^{k+1}}{6 \cdot 2^k}
            = \frac{2^{k+2} + (-1)^{k+1}}{3 \cdot 2^{k+1}}
    \end{align*}
    Finally, by the mathmetical induction, the statement is true for all nonnegative integers $n$.
\end{proof}