\begin{question}
Show that if $a \equiv b$ (mod $m$) and $c \equiv d$ (mod $m$), where $a$, $b$, $c$, $d$, and $m$ are integers with $m \geq 2$, then $a-c \equiv$ $b-d$ (mod $m$).
\end{question}

\par\noindent\rule{\textwidth}{0.5pt}

\subsubsection*{Solutions}
\indent\indent
If $a \equiv b$ (mod $m$), then $a = b + km$ for some integer $k$. Similarly, if $c \equiv d$ (mod $m$), then $c = d + lm$ for some integer $l$. Therefore, $a - c = b + km - d - lm = (b - d) + m(k - l)$, so $a - c \equiv b - d$ (mod $m$).